

Contents

§1. Lagrangian Mechanics

†a

Free Particle

1

†b

Conservative Force

1

†c

Constraint Force

1

I INTRODUCTION TO STATISTICS

§1. Measure Theory

†a

Measurable Space

3

†b

Measure and Extension Theorem

3

†c

Measure space

5

§2. Integration Theory

§1 Lagrangian Mechanics

Let us start from defining the **action**:

$$S[\mathbf{q}(t)] = \int_0^T L(\mathbf{q}, \dot{\mathbf{q}}, t) dt,$$

the **Euler-Lagrange equation** is derived from $\delta S = 0$, with an additional restriction $\delta \mathbf{q}(0) = \delta \mathbf{q}(T) = 0$:

$$\begin{aligned} \delta \int_0^T L dt &= \int_0^T (\nabla_{\mathbf{q}} L \cdot \delta \mathbf{q} + \nabla_{\dot{\mathbf{q}}} L \cdot \delta \dot{\mathbf{q}}) dt \\ &= \int_0^T \left(\nabla_{\mathbf{q}} L - \frac{d}{dt} \nabla_{\dot{\mathbf{q}}} L \right) \cdot \delta \mathbf{q} dt = 0. \end{aligned}$$

Since the choice of $\delta \mathbf{q}$ is arbitrary, we obtain the Euler-Lagrange equation (we place the highest order derivative at the beginning):

$$\frac{d}{dt} \nabla_{\dot{\mathbf{q}}} L - \nabla_{\mathbf{q}} L = \mathbf{0}. \quad (1)$$

But what is the **Lagrangian** function L ?

†a Free Particle

First, there are some symmetry about the Lagrangian:

- 1) Space translation: $L(\mathbf{q}, \dot{\mathbf{q}}, t) = L(\dot{\mathbf{q}})$.
- 2) Rotation: $L(\dot{\mathbf{q}}) = L(|\dot{\mathbf{q}}|^2)$.

In this sense:

$$2 \frac{d}{dt} L'(|\dot{\mathbf{q}}|^2) \dot{\mathbf{q}}.$$

Compare to the Newtonian Mechanics:

$$m\ddot{\mathbf{q}} = 0,$$

we make $L'(|\dot{\mathbf{q}}|^2)$ as a constant $m/2$:

$$L_{\text{free}} = T = \frac{1}{2} m |\dot{\mathbf{q}}|^2. \quad (2)$$

†b Conservative Force

In the case of conservative force:

$$m\ddot{\mathbf{r}} = \mathbf{F} = -\nabla V(\mathbf{q}).$$

Then we have

$$\frac{d}{dt} \nabla_{\dot{\mathbf{q}}} T - \nabla_{\mathbf{q}} T + \nabla V(\mathbf{q}) = \frac{d}{dt} \nabla_{\dot{\mathbf{q}}} (T - V) - \nabla_{\mathbf{q}} (T - V) = 0.$$

So we define

$$L_{\text{conserve}} = T - V = \frac{1}{2} m |\dot{\mathbf{q}}|^2 - V. \quad (3)$$

†c Constraint Force

Under the following conditions, we can use the **generalized coordinate**:

- 1) There is some holonomic constraint $f(\mathbf{q}, t)$.
- 2) The constraint force satisfies $\mathbf{F} \cdot \delta \mathbf{q} = 0$.

In Newtonian Mechanics:

$$m\ddot{\mathbf{q}} = \mathbf{F}_{\text{conserve}} + \mathbf{F}_{\text{constraint}}.$$

But in the variation of the action:

$$\begin{aligned} \delta S &= \int_0^T (m\ddot{\mathbf{q}} - \mathbf{F}_{\text{conserve}} - \mathbf{F}_{\text{constraint}}) \cdot \delta \mathbf{q} dt \\ &= \int_0^T (m\ddot{\mathbf{q}} - \mathbf{F}_{\text{conserve}}) \cdot \delta \mathbf{q} dt = 0 \end{aligned}$$

Chapter 1

Introduction to Statistics

§1 Measure Theory

†a Measurable Space

A **measurable space** is a set Ω with a σ -algebra $\mathcal{F} \subseteq 2^\Omega$, s.t.

- 1) $\Omega \in \mathcal{F}$.
- 2) $A \in \mathcal{F} \implies \Omega \setminus A \in \mathcal{F}$.
- 3) $S \subseteq \mathcal{F}, S \preceq \aleph_0 \implies \bigcup S \in \mathcal{F}$.

The σ -algebra generated by $S \subseteq 2^\Omega$, denoted by

$$\sigma \langle S \rangle,$$

is defined to be the intersection of all σ -algebra containing S^* .

§1.1 Proposition:

Let (Ω, \mathcal{F}) be a measurable space:

- 1) The definition is equivalent to replace (3) by:

$$S \subseteq \mathcal{F}, S \preceq \aleph_0 \implies \bigcap S \in \mathcal{F}.$$

- 2) $\emptyset \in \mathcal{F}$.
- 3) $A, B \in \mathcal{F} \implies A \setminus B \in \mathcal{F}$.

An **algebra** is a collection $\mathcal{F} \subseteq 2^\Omega$ s.t.

- 1) $\Omega \in \mathcal{F}$.
- 2) $A \in \mathcal{F} \implies \Omega \setminus A \in \mathcal{F}$.
- 3) $S \subseteq \mathcal{F}, S \prec \aleph_0 \implies \bigcup S \in \mathcal{F}$.

§1.2 Proposition:

Let Ω be a set, and let $\mathcal{F} \subseteq 2^\Omega$ be an algebra:

- 1) The definition is equivalent to replace (3) by:

$$S \subseteq \mathcal{F}, S \prec \aleph_0 \implies \bigcap S \in \mathcal{F}.$$

- 2) $\emptyset \in \mathcal{F}$.
- 3) $A, B \in \mathcal{F} \implies A \setminus B \in \mathcal{F}$.

§1.3 Lemma:

Let $\mathcal{F} \subseteq 2^\Omega$. Then \mathcal{F} is a σ -algebra iff. \mathcal{F} is an algebra and satisfies

$$\{A_n\}_{n \in \mathbb{N}} \subseteq \mathcal{F} \text{ increasing}^\dagger \implies \bigcup \{A_n\}_{n \in \mathbb{N}} \in \mathcal{F}.$$

A π -system is a collection $C \subseteq 2^\Omega$ s.t.

$$S \subseteq C, S \prec \aleph_0 \implies \bigcap S \in C.$$

*Notice 2^Ω is a σ -algebra containing S , the definition is well-defined.

†Which means: for every $n \in \mathbb{N}$, $A_n \subseteq A_{n+1}$.

A λ -system is a collection $\mathcal{L} \subseteq 2^\Omega$ s.t.

- 1) $\Omega \in \mathcal{L}$.
- 2) $A, B \in \mathcal{L}, A \subseteq B \implies B \setminus A \in \mathcal{L}$.
- 3) If $\{A_n\}_{n \in \mathbb{N}} \subseteq \mathcal{L}$ increasing, then $\bigcup \{A_n\}_{n \in \mathbb{N}} \in \mathcal{L}$.

The λ -system generated by $S \subseteq 2^\Omega$, denoted by

$$\lambda \langle S \rangle,$$

is defined to be the intersection of all λ -system containing S .

§1.4 Lemma: π - λ Theorem

A collection $\mathcal{F} \subseteq 2^\Omega$ is a π -system and a λ -system iff. \mathcal{F} is a σ -algebra.

§1.4.1 Corollary:

If C is a π -system, then $\lambda \langle C \rangle = \sigma \langle C \rangle$.

Proof:

Every σ -algebra is a λ -system, we have $\lambda \langle C \rangle \subseteq \sigma \langle C \rangle$.

It suffices to show $\lambda \langle C \rangle$ is a σ -algebra, i.e. $\lambda \langle C \rangle \supseteq \sigma \langle C \rangle$.

Let

$$\lambda_1 \langle C \rangle = \{A \in \lambda \langle C \rangle \mid \forall B \in C : A \cap B \in \lambda \langle C \rangle\},$$

and let

$$\lambda_2 \langle C \rangle = \{A \in \lambda \langle C \rangle \mid \forall B \in \lambda \langle C \rangle : A \cap B \in \lambda \langle C \rangle\},$$

then $\lambda_1 \langle C \rangle$ and $\lambda_2 \langle C \rangle$ are λ -systems containing C , hence $\lambda \langle C \rangle \subseteq \lambda_2 \langle C \rangle \subseteq \lambda_1 \langle C \rangle \subseteq \lambda \langle C \rangle$. Therefore, $\lambda \langle C \rangle = \lambda_2 \langle C \rangle$, $\lambda \langle C \rangle$ is a π -system, by Lem.§1.4, $\lambda \langle C \rangle$ is a σ -algebra. \square

The **Borel σ -algebra** of a t.s. (Ω, τ) is defined to be $\sigma \langle \tau \rangle$.

†b Measure and Extension Theorem

A **semialgebra** is a collection $C \subseteq 2^\Omega$ s.t.

- 1) $S \subseteq C, S \prec \aleph_0 \implies \bigcap_\Omega S \in C$.
- 2) $\forall A \in C, \exists S \subseteq C, 0 \prec S \prec \aleph_0$ pairwise disjoint[‡] s.t. $\Omega \setminus A = \bigcup S$.

A **measure** of a semialgebra $C \subseteq 2^\Omega$ is a function $\mu : C \rightarrow [0, +\infty]$ s.t.

- 1) $\mu(\emptyset) = 0$.
- 2) If $\{A_n\}_{n \in \mathbb{N}} \subseteq C$ pairwise disjoint, and if $\bigcup \{A_n\}_{n \in \mathbb{N}} \in C$, then

$$\mu \left(\bigcup \{A_n\}_{n \in \mathbb{N}} \right) = \sum_{i=0}^{\infty} \mu(A_i).$$

‡Which means: for every $i, j \in \mathbb{N}$, if $i \neq j$, then $A_i \cap A_j = \emptyset$.

§1.5 Proposition:

Let μ be a measure on a semialgebra C :

- 1) If $A, B \in C$, then $A \subseteq B \implies \mu(A) \leq \mu(B)$.
- 2) If $\{A_n\}_{n \in \mathbb{N}} \subseteq C$, and if $\bigcup \{A_n\}_{n \in \mathbb{N}} \in C$, then

$$\mu\left(\bigcup \{A_n\}_{n \in \mathbb{N}}\right) \leq \sum_{i=0}^{\infty} \mu(A_i).$$

- 3) If $\{A_n\}_{n \in \mathbb{N}} \subseteq C$ increasing, and if $\bigcup \{A_n\}_{n \in \mathbb{N}} \in C$, then

$$\mu\left(\bigcup \{A_n\}_{n \in \mathbb{N}}\right) = \lim_{n \rightarrow \infty} \mu(A_n).$$

- 4) If $\{A_n\}_{n=0}^k \subseteq C$ with $\forall 0 \leq n \leq k : \mu(A_n) < \infty$, then

$$\begin{aligned} \mu\left(\bigcup \{A_n\}_{n=0}^k\right) &= \sum_{i=0}^k \mu(A_i) - \sum_{0 \leq i < j \leq k} \mu(A_i \cap A_j) + \dots \\ &\quad + (-1)^k \mu(A_0 \cap \dots \cap A_k) \end{aligned}$$

The **algebra generated by** a semialgebra $C \subseteq 2^\Omega$, denoted by

$$\mathcal{A}\langle C \rangle,$$

is defined to be the intersection of all algebra containing C .

§1.6 Lemma:

- 1) An algebra is a semialgebra.
- 2) Let C be a semialgebra, then

$$\mathcal{A}\langle C \rangle = \left\{ A \in 2^\Omega \mid \exists \{B_i\}_{i=0}^k \subseteq C \text{ pairwise disjoint} : A = \bigcup \{B_i\}_{i=0}^k \right\}.$$

- 3) $\sigma\langle C \rangle = \sigma\langle \mathcal{A}\langle C \rangle \rangle$.

The **measure induced by** μ to the algebra $\mathcal{A}\langle C \rangle$, denoted by $\bar{\mu}$, is defined by $\bar{\mu} : \mathcal{A}\langle C \rangle \rightarrow [0, \infty]$:

$$\bar{\mu}(A) = \sum_{i=0}^k \mu(B_i),$$

where $\{B_i\}_{i=0}^k$ pairwise disjoint, and $A = \bigcup \{B_i\}_{i=0}^k$.

§1.7 Theorem:

Let μ be a measure on a semialgebra C . Then:

- 1) $\bar{\mu}$ is well-defined.
- 2) $\bar{\mu}|_C = \mu$.
- 3) $\bar{\mu}$ is a measure on $\mathcal{A}\langle C \rangle$.

Proof:

- 3) Let $\{A_n\}_{n \in \mathbb{N}} \subseteq \mathcal{A}$ be pairwise disjoint, then for each $n \in \mathbb{N}$, we have

$$A_n = \bigcup \{B_j^n \mid j \in \mathbb{N} : 0 \leq j \leq k_n \in \mathbb{N}\},$$

where $\{B_j^n \mid j \in \mathbb{N} : 0 \leq j \leq k_n \in \mathbb{N}\} \subseteq C$ pairwise disjoint. Similarly,

$$\bigcup \{A_n\}_{n \in \mathbb{N}} = \bigcup \{B_j \mid j \in \mathbb{N} : 0 \leq j \leq k \in \mathbb{N}\},$$

where $\{B_j \mid j \in \mathbb{N} : 0 \leq j \leq k \in \mathbb{N}\} \subseteq C$ pairwise disjoint. Therefore,

$$B_i = B_i \cap \bigcup \{A_n\}_{n \in \mathbb{N}} = \bigcup \{A_n \cap B_i\}_{n \in \mathbb{N}} = \bigcup \{B_j^n \cap B_i\}_{n \in \mathbb{N}, 0 \leq j \leq k_n}.$$

and

$$\mu(B_i) = \sum_{n=0}^{\infty} \sum_{j=0}^{k_n} \mu(B_j^n \cap B_i),$$

which implies

$$\bar{\mu}\left(\bigcup \{A_n\}_{n \in \mathbb{N}}\right) = \sum_{i=0}^k \sum_{n=0}^{\infty} \sum_{j=0}^{k_n} \mu(B_j^n \cap B_i) = \sum_{n=0}^{\infty} \left(\sum_{i=0}^k \sum_{j=0}^{k_n} \mu(B_j^n \cap B_i) \right).$$

While

$$A_n = A_n \cap \bigcup \{B_i\}_{0 \leq i \leq k} = \bigcup \{B_j^n \cap B_i\}_{0 \leq i \leq k, 0 \leq j \leq k_n},$$

i.e.

$$\bar{\mu}(A_n) = \sum_{i=0}^k \sum_{j=0}^{k_n} \mu(B_j^n \cap B_i).$$

Together,

$$\bar{\mu}\left(\bigcup \{A_n\}_{n \in \mathbb{N}}\right) = \sum_{n=0}^{\infty} \bar{\mu}(A_n).$$

□

The **outer measure induced by** μ , denoted by μ^* , is defined by $\mu^* : 2^\Omega \rightarrow [0, \infty]$:

$$\mu^*(A) = \inf \left\{ \sum_{n=0}^{\infty} \mu(A_n) \mid \{A_n\}_{n \in \mathbb{N}} \subseteq C : A \subseteq \bigcup \{A_n\}_{n \in \mathbb{N}} \right\}.$$

A set $A \subseteq \Omega$ is μ^* -measurable iff.

$$\forall E \subseteq \Omega : \mu^*(E) = \mu^*(E \cap A) + \mu^*(E \cap (\Omega \setminus A)).$$

The **Carathéodory σ -algebra**, denoted by

$$\mathcal{M}_{\mu^*},$$

is the collection of all μ^* -measurable sets.

§1.8 Theorem: Carathéodory Extension Theorem

Let μ be a measure on a semialgebra C :

- 1) $\mu^*|_{\mathcal{A}\langle C \rangle} = \bar{\mu}$.
- 2) If $\{A_n\}_{n \in \mathbb{N}} \subseteq 2^\Omega$, then

$$\mu^*\left(\bigcup \{A_n\}_{n \in \mathbb{N}}\right) \leq \sum_{i=0}^{\infty} \mu^*(A_i).$$

- 3) $C \subseteq \mathcal{M}_{\mu^*}$.

- 4) \mathcal{M}_{μ^*} is a σ -algebra.

- 5) $\mu^*|_{\mathcal{M}_{\mu^*}}$ is a measure.

- 6) $A \in 2^\Omega, \mu^*(A) = 0 \implies 2^A \subseteq \mathcal{M}_{\mu^*}$.

Proof:

- 1) It suffices to show $\bar{\mu}(A) \leq \mu^*(A)$.

For all $\varepsilon > 0$, there exists a collection $\{A_n\}_{n \in \mathbb{N}} \subseteq C$ s.t.

$$A \subseteq \bigcup \{A_n\}_{n \in \mathbb{N}}, \quad \sum_{n=0}^{\infty} \mu(A_n) \leq \mu^*(A) + \varepsilon.$$

Let $\{B_i\}_{i=0}^k$ pairwise disjoint s.t. $A = \bigcup \{B_i\}_{i=0}^k$, then

$$A = A \cap \bigcup \{A_n\}_{n \in \mathbb{N}} = \bigcup \{B_i \cap A_n\}_{n \in \mathbb{N}, 0 \leq i \leq k}.$$

Therefore,

$$\bar{\mu}(A) \leq \sum_{n=0}^{\infty} \sum_{i=0}^k \mu(B_i \cap A_n) = \sum_{n=0}^{\infty} \mu(A_n) \leq \mu^*(A) + \varepsilon.$$

Let $\varepsilon \rightarrow 0$, we get $\bar{\mu}(A) \leq \mu^*(A)$.

- 3) We only show $\forall E \subseteq \Omega, \forall A \in C : \mu^*(E) \geq \mu^*(E \cap A) + \mu^*(E \cap (\Omega \setminus A))$.

For all $\varepsilon > 0$, there exists a collection $\{A_n\}_{n \in \mathbb{N}} \subseteq C$ s.t.

$$E \subseteq \bigcup \{A_n\}_{n \in \mathbb{N}}, \quad \sum_{n=0}^{\infty} \mu(A_n) \leq \mu^*(E) + \varepsilon.$$

Let $\{B_i\}_{i=0}^k \subseteq C$ pairwise disjoint s.t. $\Omega \setminus A = \bigcup \{B_i\}_{i=0}^k$. Then

$$E \cap A \subseteq \bigcup \{A_n \cap A\}_{n \in \mathbb{N}}, \quad E \cap (\Omega \setminus A) \subseteq \bigcup \{A_n \cap B_i\}_{n \in \mathbb{N}, 0 \leq i \leq k}.$$

Hence

$$\begin{aligned} \mu^*(E \cap A) + \mu^*(E \cap (\Omega \setminus A)) &\leq \sum_{n=0}^{\infty} \left(\mu(A_n \cap A) + \sum_{i=0}^k \mu(A_n \cap B_i) \right) \\ &= \sum_{n=0}^{\infty} \mu(A_n) \leq \mu^*(E) + \varepsilon \end{aligned}$$

Let $\varepsilon \rightarrow 0$, we get $\mu^*(E) \geq \mu^*(E \cap A) + \mu^*(E \cap (\Omega \setminus A))$.

4) We first show that \mathcal{M}_{μ^*} is an algebra:

For convenience, we write $A^c = \Omega \setminus A$:

$$\begin{aligned} \mu^*(E) &= \mu^*(E \cap A_1) + \mu^*(E \cap A_1^c) \\ &= \mu^*(E \cap A_1 \cap A_2) + \mu^*(E \cap A_1 \cap A_2^c) \\ &\quad + \mu^*(E \cap A_1^c \cap A_2) + \mu^*(E \cap A_1^c \cap A_2^c) \end{aligned}$$

Notice that $A_1 \cup A_2 = (A_1 \cap A_2) \cup (A_1^c \cap A_2) \cup (A_1 \cap A_2^c)$, and $(A_1 \cap A_2)^c = A_1^c \cap A_2^c$. We have

$$\mu^*(E) \geq \mu^*(E \cap (A_1 \cup A_2)) + \mu^*(E \cap (A_1 \cup A_2)^c).$$

Now, we show that if $\{A_n\}_{n \in \mathbb{N}} \subseteq \mathcal{M}_{\mu^*}$ increasing, then $\bigcup \{A_n\}_{n \in \mathbb{N}} \in \mathcal{M}_{\mu^*}$.

Let $\{B_n\}_{n \in \mathbb{N}}$ be defined by

- $B_0 = A_0$,
- $B_{n+1} = A_{n+1} \setminus A_n$.

Then $\{B_n\}_{n \in \mathbb{N}} \subseteq \mathcal{M}_{\mu^*}$ pairwise disjoint, with $\bigcup \{A_n\}_{n \in \mathbb{N}} = \bigcup \{B_n\}_{n \in \mathbb{N}}$.

For $n \geq 1$:

$$\begin{aligned} \mu^*(E) &= \mu^*(E \cap A_n) + \mu^*(E \cap A_n^c) \\ &= \mu^*(E \cap A_n \cap B_n) + \mu^*(E \cap A_n \cap B_n^c) + \mu^*(E \cap A_n^c) \\ &= \mu^*(E \cap B_n) + \mu^*(E \cap A_{n-1}) + \mu^*(E \cap A_n^c) \\ &= \sum_{i=0}^n \mu^*(E \cap B_i) + \mu^*(E \cap A_n^c) \\ &\geq \sum_{i=0}^n \mu^*(E \cap B_i) + \mu^*\left(E \cap \left(\bigcup \{A_n\}_{n \in \mathbb{N}}\right)^c\right) \end{aligned}$$

Let $n \rightarrow \infty$, we have

$$\mu^*(E) \geq \mu^*\left(E \cap \bigcup \{A_n\}_{n \in \mathbb{N}}\right) + \mu^*\left(E \cap \left(\bigcup \{A_n\}_{n \in \mathbb{N}}\right)^c\right).$$

5) Let $\{B_n\}_{n \in \mathbb{N}} \subseteq \mathcal{M}_{\mu^*}$ pairwise disjoint. Let $\{A_j\}_{j \in \mathbb{N}}$ be defined by $A_j = \bigcup \{B_n\}_{n=j}^{\infty}$:

$$\begin{aligned} \mu^*(A_0) &= \mu^*(A_0 \cap B_0) + \mu^*(A_0 \cap B_0^c) \\ &= \mu^*(B_0) + \mu^*(A_1) \\ &= \mu^*(B_0) + \mu^*(B_1) + \mu^*(A_2) \\ &= \sum_{i=0}^n \mu^*(B_i) + \mu^*(A_{n+1}) \\ &\geq \sum_{i=0}^n \mu^*(B_i) \end{aligned}$$

Let $n \rightarrow \infty$, we have

$$\mu^*\left(\bigcup \{B_n\}_{n \in \mathbb{N}}\right) \geq \sum_{i=0}^{\infty} \mu^*(B_i).$$

6) Let $B \in 2^A$, then $\mu^*E \cap B = \mu^*(B) = \mu^*A = 0$, and $\mu^* \geq \mu^*(E \cap B^c)$.

†c Measure space

A **measure space** (meas.s.) is a measurable space (Ω, \mathcal{F}) with a measure on \mathcal{F}^* . The **μ -null subsets** of a m.s., denoted by \mathcal{N}_{μ} , is defined by

$$\mathcal{N}_{\mu} = \{A \subseteq \Omega \mid \exists B \supseteq A : \mu(B) = 0\}.$$

A m.s. is **complete** iff. $\mathcal{N}_{\mu} \subseteq \mathcal{F}$.

§1.9 Theorem: First Littlewood Approximation Principle

Let μ be a measure on a semialgebra C . If $A \in \mathcal{M}_{\mu^*}$, and if $\mu^*(A) < \infty$. Then for each $\varepsilon > 0$, there exists $\{B_n\}_{n=0}^k \subseteq C$ pairwise disjoint, s.t.

$$\mu^*\left(A \Delta \bigcup \{B_n\}_{n=0}^k\right) < \varepsilon,$$

where $A_1 \Delta A_2$ denote the **symmetric difference** of A_1 and A_2 , defined by $A_1 \Delta A_2 = (A_1 \cap (\Omega \setminus A_2)) \cup ((\Omega \setminus A_1) \cap A_2)$.

Proof:

§1.9.1 Corollary:

Let μ be a measure on a semialgebra C . Then:

- 1) $\mathcal{M}_{\mu^*} = \{A \Delta B \mid A \in \sigma\langle C \rangle, B \in \mathcal{N}_{\mu^*}\}$.
- 2) $\mathcal{M}_{\mu^*} = \{A \cup B \mid A \in \sigma\langle C \rangle, B \in \mathcal{N}_{\mu^*}\}$.

Proof:

§1.9.2 Corollary:

Let $(\Omega, \mathcal{F}, \mu)$ be a meas.s, and let $\tilde{\mathcal{F}} = \{A \cup B \mid A \in \mathcal{F}, B \in \mathcal{N}_{\mu}\}$.

- 1) $\tilde{\mathcal{F}}$ is a σ -algebra.
- 2) Let $\tilde{\mu} : \tilde{\mathcal{F}} \rightarrow [0, \infty]$ defined by

$$\forall A \in \mathcal{F}, \forall B \in \mathcal{N}_{\mu} : \tilde{\mu}(A \cup B) = \mu(A)$$

is well-defined measure on $\tilde{\mathcal{F}}$.

- 3) $(\Omega, \tilde{\mathcal{F}}, \tilde{\mu})$ is a complete meas.s., and $\tilde{\mu}|_{\mathcal{F}} = \mu$.

Proof:

Let μ be a measure on a semialgebra C :

- 1) μ is **finite** iff. $\mu(\Omega) < \infty$.
- 2) μ is **infinite** iff. $\mu(\Omega) = \infty$.
- 3) μ is **σ -finite** iff. $\exists \{A_n\}_{n \in \mathbb{N}} \subseteq C : \Omega = \bigcup \{A_n\}_{n \in \mathbb{N}}, \forall n \in \mathbb{N} : \mu(A_n) < \infty$.

§1.10 Theorem:

Let μ be a σ -finite measure on a semialgebra C , and let ν be a measure on $(\Omega, \sigma\langle C \rangle)$ s.t. $\nu|_C = \mu$. Then $\mu^*|_{\sigma\langle C \rangle} = \nu$.

Proof:

For the real space \mathbb{R}^k , the **standard σ -algebra**

§2 Integration Theory

Bibliography